Simplify field merging check in query conformance
The one in the spec seems too convoluted. This one uses the same
ideas as in other areas, such as collecting similar queries according to
the type in scope, etc.

src/QueryAux.v
@@ -96,6 +96,24 @@ Section QueryAux.
     end.
 
 
+  
+ Equations are_equivalent (q1 q2 : @Query Name Vals) : bool :=
+   {
+     are_equivalent (SingleField f α) (SingleField f' α') :=  (f == f') && (α == α');
+     are_equivalent (SingleField f α) (LabeledField _ f' α') :=  (f == f') && (α == α');
+     
+     are_equivalent (LabeledField _ f α) (SingleField f' α') :=  (f == f') && (α == α');
+     are_equivalent (LabeledField _ f α) (LabeledField _ f' α') :=  (f == f') && (α == α');
+
+     are_equivalent (NestedField f α _) (NestedField f' α' _) :=  (f == f') && (α == α');
+     are_equivalent (NestedField f α _) (NestedLabeledField _ f' α' _) :=  (f == f') && (α == α');
+
+     are_equivalent (NestedLabeledField _ f α _) (NestedField f' α' _) :=  (f == f') && (α == α');
+     are_equivalent (NestedLabeledField _ f α _) (NestedLabeledField _ f' α' _) :=  (f == f') && (α == α');
+
+     are_equivalent _ _ := false
+   }.
+ 
   Variable s : @wfSchema Name Vals.
 
   
@@ -255,7 +273,13 @@ Section QueryAux.
       merge_selection_sets (q :: qs) := q.(qsubqueries) ++ merge_selection_sets qs
     }.
 
-
+  Transparent merge_selection_sets qsubqueries.
+  
+  Lemma merge_selection_sets_cat (qs1 qs2 : seq (@Query Name Vals)) :
+    merge_selection_sets (qs1 ++ qs2) = merge_selection_sets qs1 ++ merge_selection_sets qs2.
+  Proof.
+      by elim: qs1 qs2 => //=; case; intros; simp merge_selection_sets => /=; rewrite H catA.
+  Qed.
   
   Lemma merged_selections_lt qs :
     qs != [::] ->
@@ -304,9 +328,59 @@ Section QueryAux.
   Admitted.
 
 
+     Equations find_fields_with_response_name : Name -> seq (@Query Name Vals) -> seq (@Query Name Vals) :=
+    {
+       find_fields_with_response_name _ [::] := [::];
+
+       find_fields_with_response_name k (InlineFragment t φ :: qs) := find_fields_with_response_name k qs;
+
+      find_fields_with_response_name k (SingleField f α :: qs)
+        with f == k :=
+        {
+        | true := SingleField f α :: find_fields_with_response_name k qs;
+        | _ := find_fields_with_response_name k qs
+        };
+      
+      find_fields_with_response_name k (LabeledField l f α :: qs)
+        with l == k :=
+        {
+        | true := LabeledField l f α :: find_fields_with_response_name k qs;
+        | _ := find_fields_with_response_name k qs
+        };
+
+      
+      find_fields_with_response_name k (NestedField f α φ :: qs)
+        with f == k :=
+        {
+        | true := NestedField f α φ :: find_fields_with_response_name k qs;
+        | _ := find_fields_with_response_name k qs
+        };
+      
+      find_fields_with_response_name k (NestedLabeledField l f α φ :: qs)
+        with l == k :=
+        {
+        | true := NestedLabeledField l f α φ  :: find_fields_with_response_name k qs;
+        | _ := find_fields_with_response_name k qs
+        }
+    }.
+
+  Lemma all_found_fields_are_fields k qs :
+    all (fun q => q.(is_field)) (find_fields_with_response_name k qs).
+  Proof.
+      by funelim (find_fields_with_response_name k qs).
+  Qed.
+
+  Lemma found_fields_leq_size k qs :
+    queries_size (find_fields_with_response_name k qs) <= queries_size qs.
+  Proof.
+      by funelim (find_fields_with_response_name k qs) => //=; simp query_size; ssromega.
+  Qed.
+
     
 End QueryAux.
 
 
+Arguments are_equivalent [Name Vals].
 Arguments filter_queries_with_label [Name Vals].
 Arguments find_queries_with_label [Name Vals].
+Arguments find_fields_with_response_name [Name Vals].
